
\begin{align}
	a^m \cdot a^n &= \left (\begin{matrix}\underbrace{a\cdot a \cdot... \cdot a}\\m 个a\end{matrix}\right) 
	\cdot \left(\begin{matrix}\underbrace{a\cdot a \cdot ...\cdot a}\\n个a\end{matrix}\right)\\
	&= \left (\begin{matrix}\underbrace{a\cdot a \cdot ...\cdot a}\\m+n 个a\end{matrix}\right) = a^{m+n}\\\\
\end{align}
\begin{align}	
	(a^m)^n = \begin{matrix} n 个 a^m\\ \overbrace{a^m\cdot a^m \cdot ...\cdot a^m}\end{matrix} 
	= a ^ {\begin{matrix} n 个 m\\ \overbrace{m+m+...+m}\end{matrix}} = a ^ {mn}
\end{align}
	